lean/Erdos9796Proof/P97/Census554/CertCheck.lean
@@ -1,3 +1,8 @@
+/-
+Copyright (c) 2026 Adam McKenna. All rights reserved.
+Released under Apache 2.0 license as described in the file LICENSE.
+Authors: Adam McKenna
+-/
 import Erdos9796Proof.P97.Census554.MotifTransfer
 import Erdos9796Proof.P97.Census554.PolyCheck
 
